x86/proofs/mldsa_poly_use_hint_88.ml
@@ -53,7 +53,7 @@ let PACK8_MERGE = prove(
 
 let mldsa_poly_use_hint_88_mc = define_assert_from_elf
  "mldsa_poly_use_hint_88_mc" "x86/mldsa/mldsa_poly_use_hint_88.o"
-(*** BYTECODE START ***)
+(* BYTECODE START *)
 [
   0xf3; 0x0f; 0x1e; 0xfa;  (* ENDBR64 *)
   0xb9; 0x7f; 0x00; 0x00; 0x00;
@@ -133,7 +133,7 @@ let mldsa_poly_use_hint_88_mc = define_assert_from_elf
                            (* JNE (Imm32 (word 4294967157)) *)
   0xc3                     (* RET *)
 ];;
-(*** BYTECODE END ***)
+(* BYTECODE END *)
 
 let mldsa_poly_use_hint_88_tmc =
   define_trimmed "mldsa_poly_use_hint_88_tmc" mldsa_poly_use_hint_88_mc;;
